scratch/dp/Monad.thy
@@ -1,5 +1,5 @@
 theory Monad
-  imports Main
+  imports Main "HOL-Library.Monad_Syntax" 
 begin
 
 datatype ('M, 'a) state = State (runState: "'M \<Rightarrow> 'a \<times> 'M")
@@ -9,13 +9,12 @@ definition return :: "'a \<Rightarrow> ('M, 'a) state" where
   "return a \<equiv> State (\<lambda>M. (a, M))"
 term 0 (**)
 
-definition bind :: "('M, 'a) state \<Rightarrow> ('a \<Rightarrow> ('M, 'b) state) \<Rightarrow> ('M, 'b) state" (infixl "\<bind>" 54) where
-  "s \<bind> k \<equiv> State (\<lambda>M. let (a, M') = runState s M in runState (k a) M')"
+definition bind :: "('M, 'a) state \<Rightarrow> ('a \<Rightarrow> ('M, 'b) state) \<Rightarrow> ('M, 'b) state" where
+  "bind s k \<equiv> State (\<lambda>M. let (a, M') = runState s M in runState (k a) M')"
 term 0 (**)
   
-abbreviation then_monad :: "('M, 'a) state \<Rightarrow> ('M, 'b) state \<Rightarrow> ('M, 'b) state" (infixl "\<then>" 54) where
-  "s \<then> s' \<equiv> s \<bind> (\<lambda>_. s')"
-term 0 (**)
+adhoc_overloading
+  Monad_Syntax.bind bind
 
 definition get :: "('M, 'M) state" where
   "get \<equiv> State (\<lambda>M. (M, M))"
@@ -24,31 +23,9 @@ definition put :: "'M \<Rightarrow> ('M, unit) state" where
   "put M \<equiv> State (\<lambda>_. ((), M))"
 term 0 (**)
   
-nonterminal exec_binds and exec_bind
-syntax
-  "_exec_block" :: "exec_binds \<Rightarrow> 'a" ("exec {//(2  _)//}" [12] 62)
-  "_exec_bind"  :: "[pttrn, 'a] \<Rightarrow> exec_bind" ("(2_ \<leftarrow>/ _)" 13)
-  "_exec_let" :: "[pttrn, 'a] \<Rightarrow> exec_bind" ("(2let _ =/ _)" [1000, 13] 13)
-  "_exec_then" :: "'a \<Rightarrow> exec_bind" ("_" [14] 13)
-  "_exec_final" :: "'a \<Rightarrow> exec_binds" ("_")
-  "_exec_cons" :: "[exec_bind, exec_binds] \<Rightarrow> exec_binds" ("_;//_" [13, 12] 12)
-
-translations
-  "_exec_block (_exec_cons (_exec_then t) (_exec_final e))"
-    \<rightleftharpoons> "CONST then_monad t e"
-  "_exec_block (_exec_cons (_exec_bind p t) (_exec_final e))"
-    \<rightleftharpoons> "CONST bind t (\<lambda>p. e)"
-  "_exec_block (_exec_cons (_exec_let p t) bs)"
-    \<rightleftharpoons> "let p = t in _exec_block bs"
-  "_exec_block (_exec_cons b (_exec_cons c cs))"
-    \<rightleftharpoons> "_exec_block (_exec_cons b (_exec_final (_exec_block (_exec_cons c cs))))"
-  "_exec_cons (_exec_let p t) (_exec_final s)"
-    \<rightleftharpoons> "_exec_final (let p = t in s)"
-  "_exec_block (_exec_final e)" \<rightharpoonup> "e"
-
-term 0 (**)
 lemma bind_assoc:
-  "(s \<bind> k0) \<bind> k1 = s \<bind> (\<lambda>a. k0 a \<bind> k1)"
+  fixes s::"('M, 'a) state" and k0 k1
+  shows "(s \<bind> k0) \<bind> k1 = s \<bind> (\<lambda>a. k0 a \<bind> k1)"
   unfolding bind_def by (auto split: prod.split)
 
 lemma left_identity:
